

1 累积量

$$F^{(k)}(s, t) = \langle \exp(se^{-i\varphi}) \rangle^{(k)} = \left\langle \sum_{m=0}^{\infty} \frac{s^m}{m!} e^{-im\varphi} \right\rangle^{(k)} \equiv \sum_{m=0}^{\infty} A_m^{(k)}(t) \frac{s^m}{m!}, A_m^{(k)}(t) = \frac{\partial^m}{\partial s^m} F^{(k)}(s, t) \Big|_{s=0}$$

$$\# : \frac{\partial}{\partial t} F^{(k)} = -(i\omega_0 + \gamma) s \frac{\partial}{\partial s} F^{(k)} - h_k s \frac{\partial^2}{\partial s^2} F^{(k)} + h_k^* s F^{(k)} + r_{j \rightarrow k} \frac{p_j}{p_k} (F^{(j)} - F^{(k)}).$$

$$\text{圆累积量: } \Psi^{(k)}(s, t) = s \frac{\partial}{\partial s} \ln F^{(k)}(s, t) \equiv \sum_{m=1}^{\infty} \varkappa_m^{(k)}(t) \frac{s^m}{m!}, \varkappa_m^{(k)}(t) = \frac{1}{m!} \frac{\partial^m}{\partial s^m} \Psi^{(k)}(s, t) \Big|_{s=0}.$$

$$\text{累积量: } \Phi^{(k)}(s, t) \equiv \ln F^{(k)}(s, t) \equiv \sum_{m=1}^{\infty} K_m^{(k)}(t) \frac{s^m}{m!}, K_m^{(k)}(t) = \frac{\partial^m}{\partial s^m} \Phi^{(k)}(s, t) \Big|_{s=0}.$$

简化记号: $F\Phi K_m$ 默认为 $F^{(k)}\Phi^{(k)}K_m^{(k)}$, $F^{(j)}\Phi^{(j)}K_m^{(j)}$ 总是保留, $A = i\omega_0 + \gamma, B = h_k, C = h_k^*, D = r_{j \rightarrow k} \frac{m_j}{m_k}$,

$$\partial_t F = -As\partial_s F - Bs\partial_s^2 F + CsF + D(F^{(j)} - F),$$

$$F = e^\Phi, \partial_s F = e^\Phi \partial_s \Phi, \partial_s^2 F = e^\Phi ((\partial_s \Phi)^2 + \partial_s^2 \Phi),$$

$$\partial_t \Phi = \frac{\partial_t F}{F} = -As \frac{\partial_s F}{F} - Bs \frac{\partial_s^2 F}{F} + Cs + D \left(\frac{F^{(j)}}{F} - 1 \right),$$

$$\# : \partial_t \Phi = -As\partial_s \Phi - Bs((\partial_s \Phi)^2 + \partial_s^2 \Phi) + Cs + D(e^{\Phi^{(j)} - \Phi^{(k)}} - 1).$$

$$\Phi = \sum_{m=1}^{\infty} K_m \frac{s^m}{m!} = K_1 s + K_2 \frac{s^2}{2!} + K_3 \frac{s^3}{3!} + \cdots,$$

$$\Phi^{(k)} = \sum_{m=1}^{\infty} K_m^{(k)} \frac{s^m}{m!}, \Phi^{(j)} = \sum_{m=1}^{\infty} K_m^{(j)} \frac{s^m}{m!},$$

$$e^{\Phi^{(j)} - \Phi^{(k)}} = \sum_{m=0}^{\infty} E_m \frac{s^m}{m!},$$

$$1 : \partial_t \Phi = \sum_{m=1}^{\infty} \dot{K}_m \frac{s^m}{m!}, \partial_s \Phi = \sum_{m=1}^{\infty} K_m \frac{s^{m-1}}{(m-1)!} = \sum_{n=0}^{\infty} K_{n+1} \frac{s^n}{n!}, 2 : s\partial_s \Phi = \sum_{m=1}^{\infty} m K_m \frac{s^m}{m!}.$$

$$\left(\sum_{n=0}^{\infty} a_n \frac{s^n}{n!} \right) \left(\sum_{n=0}^{\infty} b_n \frac{s^n}{n!} \right) = \sum_{n=0}^{\infty} c_n \frac{s^n}{n!}, \text{ where } c_n = \sum_{r=0}^n \binom{n}{r} a_r b_{n-r},$$

$$(\partial_s \Phi)^2 = \left(\sum_{n=0}^{\infty} K_{n+1} \frac{s^n}{n!} \right) \left(\sum_{n=0}^{\infty} K_{n+1} \frac{s^n}{n!} \right) = \sum_{n=0}^{\infty} \left[\sum_{r=0}^n \binom{n}{r} K_{r+1} K_{n-r+1} \right] \frac{s^n}{n!},$$

$$3 : s(\partial_s \Phi)^2 = \sum_{m=1}^{\infty} \left[m \sum_{r=0}^{m-1} \binom{m-1}{r} K_{r+1} K_{m-r} \right] \frac{s^m}{m!}.$$

$$4 : s\partial_s^2 \Phi = s \sum_{m=2}^{\infty} K_m \frac{s^{m-2}}{(m-2)!} = \sum_{n=2}^{\infty} K_n \frac{s^{n-1}}{(n-2)!} = \sum_{m=1}^{\infty} m K_{m+1} \frac{s^m}{m!}.$$

5 : CompleteBellPolynomials :

$$\text{Define } H = \Phi^{(j)} - \Phi^{(k)} = \sum_{m=1}^{\infty} \Delta K_m \frac{s^m}{m!}, e^H = \sum_{m=0}^{\infty} E_m \frac{s^m}{m!},$$

$$\begin{aligned}
\partial_s e^H &= H' \cdot e^H, H' = \sum_{m=1}^{\infty} \Delta K_m \frac{s^{m-1}}{(m-1)!} \\
H' \cdot e^H &= \left(\sum_{n=0}^{\infty} \Delta K_{n+1} \frac{s^n}{n!} \right) \left(\sum_{m=0}^{\infty} E_m \frac{s^m}{m!} \right) = \sum_{j=0}^{\infty} \left(\sum_{k=0}^j \binom{j}{k} \Delta K_{k+1} E_{j-k} \right) \frac{s^j}{j!}, \\
\partial_s e^H &= \sum_{m=1}^{\infty} E_m \frac{s^{m-1}}{(m-1)!} = \sum_{j=0}^{\infty} E_{j+1} \frac{s^j}{j!}, \\
E_{j+1} &= \sum_{k=0}^j \binom{j}{k} \Delta K_{k+1} E_{j-k}, j+1 = m, r = m-1-k \\
E_m &= \sum_{r=0}^{m-1} \binom{m-1}{r} E_r \cdot \Delta K_{m-r}, E_0 = 1, \\
e^{\Phi^{(j)} - \Phi^{(k)}} - 1 &= \sum_{m=1}^{\infty} E_m \frac{s^m}{m!}.
\end{aligned}$$

$$\# : \dot{K}_m = -mAK_m - mB \left[\sum_{r=0}^{m-1} \binom{m-1}{r} K_{r+1} K_{m-r} + K_{m+1} \right] + C\delta_{m,1} + DE_m,$$

$$\text{where } E_m = \sum_{r=0}^{m-1} \binom{m-1}{r} E_r \Delta K_{m-r}, E_0 = 1, \Delta K_{m-r} = K_{m-r}^{(j)} - K_{m-r}^{(k)}.$$

$$\begin{cases} E_1 = \Delta K_1, \\ E_2 = \Delta K_2 + (\Delta K_1)^2, \\ E_3 = \Delta K_3 + 3\Delta K_1 \Delta K_2 + (\Delta K_1)^3 \\ \dots \end{cases}$$

$$\text{Define } \kappa_m = \frac{K_m}{(m-1)!},$$

$$\binom{m}{r} = \frac{m!}{r!(m-r)!}, \binom{m-1}{r} = \frac{(m-1)!}{r!(m-1-r)!},$$

$$\kappa_{m-r} = \frac{K_{m-r}}{(m-r-1)!}, E_m = \sum_{r=0}^{m-1} \frac{E_r}{r!} (\kappa_{m-r}^{(j)} - \kappa_{m-r}^{(k)})$$

$$\# : \dot{\kappa}_m = -mA\kappa_m - mB \left(\sum_{r=0}^{m-1} \kappa_{r+1} \kappa_{m-r} + m\kappa_{m+1} \right) + C\delta_{m,1} + DE_m,$$

$$\text{where } E_m = \sum_{r=0}^{m-1} \frac{E_r}{r!} \Delta \kappa_{m-r}, \Delta \kappa_{m-r} = \kappa_{m-r}^{(j)} - \kappa_{m-r}^{(k)}, E_0 = 1.$$

$$\begin{cases} E_1 = \Delta \kappa_1, \\ E_2 = \Delta \kappa_2 + (\Delta \kappa_1)^2 \\ E_3 = \Delta \kappa_3 + \frac{2}{3} \Delta \kappa_1 \Delta \kappa_2 + \frac{1}{2} (\Delta \kappa_1)^3 \\ \dots \end{cases}$$

$$\begin{aligned}\mathcal{E}_m &= \frac{E_m}{(m-1)!} \\ \mathcal{E}_m (m-1)! &= \sum_{r=0}^{m-1} \frac{\mathcal{E}_r}{r} \Delta \kappa_{m-r}\end{aligned}$$